Proof_subtype/vars.v
@@ -1,0 +1,20 @@
+Definition id := nat.
+
+(* locally nameless for binders in terms and types/qualifiers *)
+Inductive var : Type :=
+| varF : id -> var (* free var (deBruijn level) *)
+| varB : id -> var (* locally-bound variable (deBruijn index) *)
+.
+
+Notation "# i" := (varB i) (at level 0, right associativity).
+Notation "$ i" := (varF i) (at level 0, right associativity).
+
+
+
+Definition f := nat.  (* field *)
+
+Definition m := nat.  (* method *)
+
+Definition l := nat.  (* locations *)
+
+Definition cn := nat.  (* class name *)
